ViperBoogieEndToEnd.thy
@@ -2,10 +2,6 @@ theory ViperBoogieEndToEnd
 imports StmtRel
 begin
 
-definition vpr_store_well_typed :: "('a \<Rightarrow> abs_type) \<Rightarrow> vtyp list \<Rightarrow> 'a store \<Rightarrow> bool"
-  where "vpr_store_well_typed A vs \<sigma> \<equiv> \<forall>i. 0 \<le> i \<and> i < length vs \<longrightarrow> 
-                         map_option (\<lambda>v. get_type A v) (\<sigma> i) = Some (vs ! i)"
-
 definition vpr_method_correct_total :: "'a total_context \<Rightarrow> ('a full_total_state \<Rightarrow> bool) \<Rightarrow> method_decl \<Rightarrow> bool" where
   "vpr_method_correct_total ctxt R mdecl \<equiv>
         \<forall>mbody. method_decl.body mdecl = Some mbody \<longrightarrow>
@@ -16,50 +12,7 @@ definition vpr_method_correct_total :: "'a total_context \<Rightarrow> ('a full_
                   is_empty_total_full \<omega> \<longrightarrow>
                   red_stmt_total ctxt R (nth_option (method_decl.args mdecl @ method_decl.rets mdecl)) mbody \<omega> r \<longrightarrow> r \<noteq> RFailure)"
 
-text \<open>Accesses to old expressions are represented via labeled old expressions with label \<^const>\<open>old_label\<close>.\<close>
-
-definition vpr_postcondition_framed :: "'a total_context \<Rightarrow> ('a full_total_state \<Rightarrow> bool) \<Rightarrow> assertion \<Rightarrow> 'a full_total_state \<Rightarrow> 'a store \<Rightarrow> bool"
-  where "vpr_postcondition_framed ctxt R postcondition \<omega>pre \<sigma> \<equiv>
-                   (\<forall>mh. total_heap_well_typed (program_total ctxt) (absval_interp_total ctxt) (get_hh_total mh) \<longrightarrow>
-                         wf_mask_simple (get_mh_total mh) \<longrightarrow>
-                         assertion_framing_state ctxt R postcondition
-                                 \<lparr> get_store_total = \<sigma>,
-                                 \<comment>\<open>old state given by state that satisfies precondition\<close>
-                                  get_trace_total = [old_label \<mapsto> get_total_full \<omega>pre], 
-                                  get_total_full = mh \<rparr>
-                )"
-
-definition vpr_method_body_correct :: "'a total_context \<Rightarrow> ('a full_total_state \<Rightarrow> bool) \<Rightarrow> method_decl \<Rightarrow> 'a full_total_state \<Rightarrow> bool"
-  where "vpr_method_body_correct ctxt R mdecl \<omega>pre \<equiv>
-            (\<forall>rbody. red_stmt_total ctxt R 
-                                (nth_option (method_decl.args mdecl @ method_decl.rets mdecl))
-                                (Seq (the (method_decl.body mdecl)) (Exhale (method_decl.post mdecl)))
-                                (update_trace_total \<omega>pre (Map.empty(old_label \<mapsto> get_total_full \<omega>pre))) 
-                                rbody \<longrightarrow> rbody \<noteq> RFailure)
-                        \<comment>\<open>  (rbody \<noteq> RFailure \<and> 
-                            (\<forall>\<omega>body. rbody = RNormal \<omega>body \<longrightarrow> 
-                                (\<forall> rpost. red_exhale ctxt R \<omega>body (method_decl.post mdecl) \<omega>body rpost \<longrightarrow> rpost \<noteq> RFailure)
-                            )
-                          )\<close>
-                "
-
-definition vpr_method_correct_total_2 :: "'a total_context \<Rightarrow> ('a full_total_state \<Rightarrow> bool) \<Rightarrow> method_decl \<Rightarrow> bool" where
-  "vpr_method_correct_total_2 ctxt R mdecl \<equiv>
-        \<forall>mbody. method_decl.body mdecl = Some mbody \<longrightarrow>
-         (\<forall>(\<omega> :: 'a full_total_state) rpre. 
-            vpr_store_well_typed (absval_interp_total ctxt) (method_decl.args mdecl @ method_decl.rets mdecl) (get_store_total \<omega>) \<longrightarrow>
-            total_heap_well_typed (program_total ctxt) (absval_interp_total ctxt) (get_hh_total_full \<omega>) \<longrightarrow>
-            is_empty_total_full \<omega> \<longrightarrow>
-            red_inhale ctxt R (method_decl.pre mdecl) \<omega> rpre \<longrightarrow>
-            (
-              rpre \<noteq> RFailure \<and>
-              (\<forall>\<omega>pre. rpre = RNormal \<omega>pre \<longrightarrow> 
-                \<comment>\<open>\<^term>\<open>get_store_total \<omega>\<close> should be equal to \<^term>\<open>get_store_total \<omega>pre\<close> since inhale does not change the store.\<close>
-                vpr_postcondition_framed ctxt R (method_decl.post mdecl) \<omega>pre (get_store_total \<omega>) \<and>
-                vpr_method_body_correct ctxt R mdecl \<omega>pre
-              )
-            )
-         )"
+text \<open>Accesses to old expressions are represented via labeled old expressions with label \<^const>\<open>old_label\<close>.\<close>  
 
 lemma valid_configuration_not_failure:
   assumes "valid_configuration A \<Lambda> \<Gamma> \<Omega> posts bb cont state"
